修改了一些验证条件，目前还剩app list box 和sll2array没有完成

TheoryTask/qcp-binary-democases/QCP_examples/sll_lib.c
@@ -1,249 +1,258 @@
-#include "verification_stdlib.h"
-#include "verification_list.h"
 #include "sll_project_def.h"
+#include "verification_list.h"
+#include "verification_stdlib.h"
 
-struct sll * nil_list()
+struct sll *nil_list()
 /*@ Require emp
     Ensure sll(__return, nil)
 */
 {
-    return (struct sll *) 0;
+  return (struct sll *)0;
 }
-    
-    struct sll * new_list_node()
+
+struct sll *new_list_node()
     /*@ Require emp
     Ensure __return != 0 &&
            store(&(__return -> data), 0) *
            store(&(__return -> next), 0)
 */;
 
-struct sll * cons_list(unsigned int data, struct sll * next)
+struct sll *cons_list(unsigned int data, struct sll *next)
 /*@ With l
     Require sll(next, l)
     Ensure sll(__return, cons(data, l))
 */
 {
-    struct sll * node = new_list_node();
-    node -> data = data;
-    node -> next = next;
-    return node;
+  struct sll *node = new_list_node();
+  node->data = data;
+  node->next = next;
+  return node;
 }
 
-void free_list_node(struct sll * p)
-/*@ Require exists d n, p -> data == d && p -> next == n && emp
-    Ensure emp
-*/;
+void free_list_node(struct sll *p)
+    /*@ Require exists d n, store(&(p -> data), d) * store(&(p -> next), n)
+        Ensure emp
+    */
+    ;
 
-void free_list(struct sll * head)
+void free_list(struct sll *head)
 /*@ With l
     Require sll(head, l)
     Ensure emp
 */
 {
-    /*@ Inv exists l_rest, sll(head, l_rest) */
-    while (head) {
-        /*@ exists l_rest, head != 0 && sll(head, l_rest)
-            which implies
-            exists l_rest_new, l_rest == cons(head->data, l_rest_new) && sll(head->next, l_rest_new)
-        */
-        struct sll * tmp = head;
-        head = head -> next;
-        free_list_node(tmp);
-    }
+  /*@ Inv exists l_rest, sll(head, l_rest) */
+  while (head) {
+    /*@ exists l_rest, head != 0 && sll(head, l_rest)
+        which implies
+        exists l_rest_new, l_rest == cons(head->data, l_rest_new) &&
+       sll(head->next, l_rest_new)
+    */
+    struct sll *tmp = head;
+    head = head->next;
+    free_list_node(tmp);
+  }
 }
 
-void map_list(struct sll * head, unsigned int x)
+void map_list(struct sll *head, unsigned int x)
 /*@ With l
     Require sll(head, l)
     Ensure sll(head, map_mult(x, l))
 */
 {
-    struct sll * p;
-    /*@ Inv exists l1 l2, l == app(l1, l2) && 
-            sllseg(head, p, map_mult(x, l1)) * sll(p, l2)
+  struct sll *p;
+  /*@ Inv exists l1 l2, l == app(l1, l2) &&
+          sllseg(head@pre, p, map_mult(x@pre, l1)) * sll(p, l2) &&
+          head == head@pre && x == x@pre
+  */
+  for (p = head; p != (struct sll *)0; p = p->next) {
+    /*@ exists l1 l2, l == app(l1, l2) &&
+            sllseg(head, p, map_mult(x, l1)) * sll(p, l2) &&
+            p != 0
+        which implies
+        exists l2_new, l2 == cons(p->data, l2_new) &&
+            sllseg(head, p, map_mult(x, l1)) * sll(p->next, l2_new)
     */
-    for (p = head; p != (struct sll *) 0; p = p -> next) {
-        /*@ exists l1 l2, l == app(l1, l2) && 
-                sllseg(head, p, map_mult(x, l1)) * sll(p, l2) &&
-                p != 0
-            which implies
-            exists l2_new, l2 == cons(p->data, l2_new) && 
-                sllseg(head, p, map_mult(x, l1)) * sll(p->next, l2_new)
-        */
-        p -> data = x * p -> data;
-    }
-}   
+    p->data = x * p->data;
+  }
+}
 
-struct sllb * new_sllb()
-/*@ Require emp
-    Ensure __return != 0 &&
-           store(&(__return -> head), 0) *
-           store(&(__return -> ptail), 0)
-*/;
+struct sllb *new_sllb()
+    /*@ Require emp
+        Ensure __return != 0 &&
+               store(&(__return -> head), 0) *
+               store(&(__return -> ptail), 0)
+    */
+    ;
 
-struct sllb * nil_list_box()
+struct sllb *nil_list_box()
 /*@ Require emp
     Ensure sllb(__return, nil)
 */
 {
-    struct sllb * box = new_sllb();
-    box -> head = nil_list();
-    box -> ptail  = & box -> head;
-    /*@ box -> head == 0 && box -> ptail == &(box -> head) && sll(0, nil)
-        which implies
-        sllb(box, nil)
-    */
-    return box;
+  struct sllb *box = new_sllb();
+  box->head = nil_list();
+  box->ptail = &box->head;
+  /*@ box != 0 && box -> head == 0 && box -> ptail == &(box -> head) && sll(0,
+     nil) which implies sllb(box, nil)
+  */
+  return box;
 }
 
-struct sllb * cons_list_box(unsigned int data, struct sllb * box)
+struct sllb *cons_list_box(unsigned int data, struct sllb *box)
 /*@ With l
     Require sllb(box, l)
     Ensure sllb(__return, cons(data, l))
 */
 {
-    /*@ sllb(box, l)
-        which implies
-        exists h pt,
-            box -> head == h && box -> ptail == pt && sll(h, l)
-    */
-    box -> head = cons_list(data, box -> head);
-    if (box -> ptail == & box -> head)
-    {
-        box -> ptail = & (box -> head -> next);
-    }
-    return box;
+  /*@ sllb(box, l)
+      which implies
+      exists h pt,
+          box != 0 && box -> head == h && box -> ptail == pt &&
+          sll(h, l)
+  */
+  box->head = cons_list(data, box->head);
+  if (box->ptail == &box->head) {
+    box->ptail = &(box->head->next);
+  }
+  return box;
 }
 
-struct sllb * map_list_box(struct sllb * box, unsigned int x)
+struct sllb *map_list_box(struct sllb *box, unsigned int x)
 /*@ With l
     Require sllb(box, l)
     Ensure sllb(__return, map_mult(x, l))
 */
 {
-    /*@ sllb(box, l)
-        which implies
-        exists h pt, box -> head == h && box -> ptail == pt && sll(h, l)
-    */
-    map_list(box -> head, x);
-    return box;
+  /*@ sllb(box, l)
+      which implies
+      exists h pt, box != 0 && box -> head == h && box -> ptail == pt && sll(h,
+     l)
+  */
+  map_list(box->head, x);
+  return box;
 }
 
-void free_sllb(struct sllb * p)
-/*@ Require exists x y, p -> head == x && p -> ptail == y && emp
-    Ensure emp
-*/;
+void free_sllb(struct sllb *p)
+    /*@ Require exists x y, p -> head == x && p -> ptail == y && emp
+        Ensure emp
+    */
+    ;
 
-void free_list_box(struct sllb * box)
+void free_list_box(struct sllb *box)
 /*@ With l
     Require sllb(box, l)
     Ensure emp
 */
 {
-    /*@ sllb(box, l)
-        which implies
-        exists h pt, box -> head == h && box -> ptail == pt && sll(h, l)
-    */
-    free_list(box -> head);
-    free_sllb(box);
+  /*@ sllb(box, l)
+      which implies
+      exists h pt, box -> head == h && box -> ptail == pt && sll(h, l)
+  */
+  free_list(box->head);
+  free_sllb(box);
 }
 
-struct sllb * app_list_box(struct sllb * b1, struct sllb * b2)
+struct sllb *app_list_box(struct sllb *b1, struct sllb *b2)
 /*@ With l1 l2
     Require sllb(b1, l1) * sllb(b2, l2)
     Ensure sllb(__return, app(l1, l2))
 */
 {
-    /*@ sllb(b1, l1) * sllb(b2, l2)
-        which implies
-        exists h1 pt1 h2 pt2,
-            b1 -> head == h1 && b1 -> ptail == pt1 &&
-            b2 -> head == h2 && b2 -> ptail == pt2 &&
-            sllbseg(&(b1 -> head), pt1, l1) * store(pt1, struct sll *, 0) *
-            sllbseg(&(b2 -> head), pt2, l2) * store(pt2, struct sll *, 0)
-    */
-    struct sll * h2 = b2 -> head;
-    struct sll ** pt2 = b2 -> ptail;
-    * (b1 -> ptail) = h2;
-    if (h2 != (struct sll *) 0)
-    {
-        b1 -> ptail = pt2;
-    }
-    free_sllb(b2);
-    return b1;
+  /*@ sllb(b1, l1) * sllb(b2, l2)
+      which implies
+      exists h1 pt1 h2 pt2,
+          b1 -> head == h1 && b1 -> ptail == pt1 &&
+          b2 -> head == h2 && b2 -> ptail == pt2 &&
+          sllbseg(&(b1 -> head), pt1, l1) * store(pt1, struct sll *, 0) *
+          sllbseg(&(b2 -> head), pt2, l2) * store(pt2, struct sll *, 0)
+  */
+  struct sll *h2 = b2->head;
+  struct sll **pt2 = b2->ptail;
+  *(b1->ptail) = h2;
+  if (h2 != (struct sll *)0) {
+    b1->ptail = pt2;
+  }
+  free_sllb(b2);
+  return b1;
 }
 
-unsigned int sll_length(struct sll * head)
+unsigned int sll_length(struct sll *head)
 /*@ With l
     Require sll(head, l) && Zlength(l) <= 2147483647
     Ensure __return == Zlength(l) && sll(head@pre, l)
 */
 {
-    unsigned int len = 0;
-    /*@ Inv exists l1 l2,
-            l == app(l1, l2) &&
-            len == Zlength(l1) &&
-            sllseg(head@pre, head, l1) * sll(head, l2)
-    */
-    while (head) {
-        /*@ exists l2, head != 0 && sll(head, l2)
-            which implies
-            exists l3, l2 == cons(head -> data, l3) && sll(head -> next, l3)
-        */
-        ++ len;
-        head = head -> next;
-    }
-    return len;
-}
-
-unsigned int * new_uint_array(unsigned int n)
-/*@ With n0
-    Require n == n0 && emp
-    Ensure UIntArray::undef_ceil(__return, 0, n0)
-*/;
-
-unsigned int sll2array(struct sll * head, unsigned int ** out_array)
-/*@ With l
-    Require sll(head, l) && Zlength(l) <= 2147483647 && undef_data_at(out_array, unsigned int *)
-    Ensure exists arr_ret, sll(head@pre, l) && store(out_array@pre, unsigned int *, arr_ret) && UIntArray::full_shape(arr_ret, Zlength(l))
-*/
-{
-    unsigned int len = sll_length(head);
-    unsigned int * arr = new_uint_array(len);
-    unsigned int i = 0;
-    struct sll * p = head;
-    /*@ Inv exists l1 l2,
-            l == app(l1, l2) &&
-            i == Zlength(l1) &&
-            len == Zlength(l) &&
-            0 <= i && i <= len &&
-            sllseg(head@pre, p, l1) * sll(p, l2) *
-            UIntArray::ceil_shape(arr, 0, i) * UIntArray::undef_ceil(arr, i, len)
-    */
-    while (p) {
-        /*@ exists l1 l2, l == app(l1, l2) && p != 0 && i < len && sll(p, l2) *
-                sllseg(head@pre, p, l1) * UIntArray::ceil_shape(arr, 0, i) * UIntArray::undef_ceil(arr, i, len)
-            which implies
-            exists l3, l2 == cons(p -> data, l3) && i < len && sll(p -> next, l3) *
-                sllseg(head@pre, p, l1) * UIntArray::ceil_shape(arr, 0, i) * UIntArray::undef_ceil(arr, i, len)
-        */
-        arr[i] = p -> data;
-        i = i + 1;
-        p = p -> next;
-    }
-    * out_array = arr;
-    return len;
-}
-
-unsigned int sllb2array(struct sllb * box, unsigned int ** out_array)
-/*@ With l
-    Require sllb(box, l) && Zlength(l) <= 2147483647 && undef_data_at(out_array, unsigned int *)
-    Ensure exists arr_ret, sllb(box@pre, l) && store(out_array@pre, unsigned int *, arr_ret) && UIntArray::full_shape(arr_ret, Zlength(l))
-*/
-{
-    /*@ sllb(box, l)
+  unsigned int len = 0;
+  /*@ Inv exists l1 l2,
+          l == app(l1, l2) &&
+          len == Zlength(l1) &&
+          sllseg(head@pre, head, l1) * sll(head, l2)
+  */
+  while (head) {
+    /*@ exists l2, head != 0 && sll(head, l2)
         which implies
-        exists h pt, box -> head == h && box -> ptail == pt && sll(h, l)
+        exists l3, l2 == cons(head -> data, l3) && sll(head -> next, l3)
     */
-    return sll2array(box -> head, out_array);
+    ++len;
+    head = head->next;
+  }
+  return len;
+}
+
+unsigned int *new_uint_array(unsigned int n)
+    /*@ With n0
+        Require n == n0 && emp
+        Ensure UIntArray::undef_ceil(__return, 0, n0)
+    */
+    ;
+
+unsigned int sll2array(struct sll *head, unsigned int **out_array)
+/*@ With l
+    Require sll(head, l) && Zlength(l) <= 2147483647 && undef_data_at(out_array,
+   unsigned int *) Ensure exists arr_ret, sll(head@pre, l) &&
+   store(out_array@pre, unsigned int *, arr_ret) &&
+   UIntArray::full_shape(arr_ret, Zlength(l))
+*/
+{
+  unsigned int len = sll_length(head);
+  unsigned int *arr = new_uint_array(len);
+  unsigned int i = 0;
+  struct sll *p = head;
+  /*@ Inv exists l1 l2,
+          l == app(l1, l2) &&
+          i == Zlength(l1) &&
+          len == Zlength(l) &&
+          0 <= i && i <= len &&
+          sllseg(head@pre, p, l1) * sll(p, l2) *
+          UIntArray::ceil_shape(arr, 0, i) * UIntArray::undef_ceil(arr, i, len)
+  */
+  while (p) {
+    /*@ exists l1 l2, l == app(l1, l2) && p != 0 && i < len && sll(p, l2) *
+            sllseg(head@pre, p, l1) * UIntArray::ceil_shape(arr, 0, i) *
+       UIntArray::undef_ceil(arr, i, len) which implies exists l3, l2 == cons(p
+       -> data, l3) && i < len && sll(p -> next, l3) * sllseg(head@pre, p, l1) *
+       UIntArray::ceil_shape(arr, 0, i) * UIntArray::undef_ceil(arr, i, len)
+    */
+    arr[i] = p->data;
+    i = i + 1;
+    p = p->next;
+  }
+  *out_array = arr;
+  return len;
+}
+
+unsigned int sllb2array(struct sllb *box, unsigned int **out_array)
+/*@ With l
+    Require sllb(box, l) && Zlength(l) <= 2147483647 && undef_data_at(out_array,
+   unsigned int *) Ensure exists arr_ret, sllb(box@pre, l) &&
+   store(out_array@pre, unsigned int *, arr_ret) &&
+   UIntArray::full_shape(arr_ret, Zlength(l))
+*/
+{
+  /*@ sllb(box, l)
+      which implies
+      exists h pt, box -> head == h && box -> ptail == pt && sll(h, l)
+  */
+  return sll2array(box->head, out_array);
 }
