TheoryTask/qcp-binary-democases/SeparationLogic/examples/sll_project_goal.v
@@ -14,13 +14,13 @@ Local Open Scope Z_scope.
 Local Open Scope sets.
 Local Open Scope string.
 Local Open Scope list.
-Import naive_C_Rules.
 Require Import sll_project_lib.
+Import naive_C_Rules.
 Local Open Scope sac.
-Require Import common_strategy_goal.
-Require Import common_strategy_proof.
-Require Import sll_project_strategy_goal.
-Require Import sll_project_strategy_proof.
+From SimpleC.EE Require Import sll_project_strategy_goal.
+From SimpleC.EE Require Import sll_project_strategy_proof.
+From SimpleC.EE Require Import common_strategy_goal.
+From SimpleC.EE Require Import common_strategy_proof.
 
 (*----- Function nil_list -----*)
 
@@ -135,13 +135,13 @@ forall (l_rest: (@list Z)) (head: Z) ,
 (*----- Function map_list -----*)
 
 Definition map_list_safety_wit_1 := 
-forall (l: (@list Z)) (head: Z) (p: Z) (x: Z) (l1: (@list Z)) (l2: (@list Z)) ,
+forall (x_pre: Z) (head_pre: Z) (l: (@list Z)) (p: Z) (l1: (@list Z)) (l2: (@list Z)) ,
   [| (l = (app (l1) (l2))) |]
-  &&  ((( &( "x" ) )) # UInt  |-> x)
-  **  ((( &( "p" ) )) # Ptr  |-> p)
-  **  ((( &( "head" ) )) # Ptr  |-> head)
-  **  (sllseg head p (map_mult (x) (l1)) )
+  &&  ((( &( "p" ) )) # Ptr  |-> p)
+  **  (sllseg head_pre p (map_mult (x_pre) (l1)) )
   **  (sll p l2 )
+  **  ((( &( "head" ) )) # Ptr  |-> head_pre)
+  **  ((( &( "x" ) )) # UInt  |-> x_pre)
 |--
   [| (0 <= INT_MAX) |] 
   &&  [| ((INT_MIN) <= 0) |]
@@ -158,57 +158,57 @@ forall (x_pre: Z) (head_pre: Z) (l: (@list Z)) ,
 .
 
 Definition map_list_entail_wit_2 := 
-forall (l: (@list Z)) (head: Z) (p: Z) (x: Z) (l1_2: (@list Z)) (l2_2: (@list Z)) (p_next: Z) (p_data: Z) (l2_new: (@list Z)) ,
+forall (x_pre: Z) (head_pre: Z) (l: (@list Z)) (p: Z) (l1_2: (@list Z)) (l2_2: (@list Z)) (p_next: Z) (p_data: Z) (l2_new: (@list Z)) ,
   [| (l2_2 = (cons (p_data) (l2_new))) |] 
   &&  [| (p <> 0) |] 
   &&  [| (l = (app (l1_2) (l2_2))) |]
-  &&  ((&((p)  # "sll" ->ₛ "data")) # UInt  |-> (unsigned_last_nbits ((x * p_data )) (32)))
-  **  (sllseg head p (map_mult (x) (l1_2)) )
+  &&  ((&((p)  # "sll" ->ₛ "data")) # UInt  |-> (unsigned_last_nbits ((x_pre * p_data )) (32)))
+  **  (sllseg head_pre p (map_mult (x_pre) (l1_2)) )
   **  ((&((p)  # "sll" ->ₛ "next")) # Ptr  |-> p_next)
   **  (sll p_next l2_new )
 |--
   EX (l1: (@list Z))  (l2: (@list Z)) ,
   [| (l = (app (l1) (l2))) |]
-  &&  (sllseg head p_next (map_mult (x) (l1)) )
+  &&  (sllseg head_pre p_next (map_mult (x_pre) (l1)) )
   **  (sll p_next l2 )
 .
 
 Definition map_list_return_wit_1 := 
-forall (x_pre: Z) (head_pre: Z) (l: (@list Z)) (head: Z) (p: Z) (x: Z) (l1: (@list Z)) (l2: (@list Z)) ,
+forall (x_pre: Z) (head_pre: Z) (l: (@list Z)) (p: Z) (l1: (@list Z)) (l2: (@list Z)) ,
   [| (p = 0) |] 
   &&  [| (l = (app (l1) (l2))) |]
-  &&  (sllseg head p (map_mult (x) (l1)) )
+  &&  (sllseg head_pre p (map_mult (x_pre) (l1)) )
   **  (sll p l2 )
 |--
   (sll head_pre (map_mult (x_pre) (l)) )
 .
 
 Definition map_list_partial_solve_wit_1_pure := 
-forall (l: (@list Z)) (head: Z) (p: Z) (x: Z) (l1: (@list Z)) (l2: (@list Z)) ,
+forall (x_pre: Z) (head_pre: Z) (l: (@list Z)) (p: Z) (l1: (@list Z)) (l2: (@list Z)) ,
   [| (p <> 0) |] 
   &&  [| (l = (app (l1) (l2))) |]
-  &&  ((( &( "x" ) )) # UInt  |-> x)
-  **  ((( &( "p" ) )) # Ptr  |-> p)
-  **  ((( &( "head" ) )) # Ptr  |-> head)
-  **  (sllseg head p (map_mult (x) (l1)) )
+  &&  ((( &( "p" ) )) # Ptr  |-> p)
+  **  (sllseg head_pre p (map_mult (x_pre) (l1)) )
   **  (sll p l2 )
+  **  ((( &( "head" ) )) # Ptr  |-> head_pre)
+  **  ((( &( "x" ) )) # UInt  |-> x_pre)
 |--
   [| (l = (app (l1) (l2))) |] 
   &&  [| (p <> 0) |]
 .
 
 Definition map_list_partial_solve_wit_1_aux := 
-forall (l: (@list Z)) (head: Z) (p: Z) (x: Z) (l1: (@list Z)) (l2: (@list Z)) ,
+forall (x_pre: Z) (head_pre: Z) (l: (@list Z)) (p: Z) (l1: (@list Z)) (l2: (@list Z)) ,
   [| (p <> 0) |] 
   &&  [| (l = (app (l1) (l2))) |]
-  &&  (sllseg head p (map_mult (x) (l1)) )
+  &&  (sllseg head_pre p (map_mult (x_pre) (l1)) )
   **  (sll p l2 )
 |--
   [| (l = (app (l1) (l2))) |] 
   &&  [| (p <> 0) |] 
   &&  [| (p <> 0) |] 
   &&  [| (l = (app (l1) (l2))) |]
-  &&  (sllseg head p (map_mult (x) (l1)) )
+  &&  (sllseg head_pre p (map_mult (x_pre) (l1)) )
   **  (sll p l2 )
 .
 
@@ -265,7 +265,8 @@ forall (retval: Z) (retval_2: Z) ,
   **  ((&((retval)  # "sllb" ->ₛ "ptail")) # Ptr  |-> &((retval)  # "sllb" ->ₛ "head"))
   **  ((( &( "box" ) )) # Ptr  |-> retval)
 |--
-  [| (0 = 0) |] 
+  [| (retval <> 0) |] 
+  &&  [| (0 = 0) |] 
   &&  [| (&((retval)  # "sllb" ->ₛ "head") = &((retval)  # "sllb" ->ₛ "head")) |]
 .
 
@@ -276,7 +277,8 @@ forall (retval: Z) (retval_2: Z) ,
   **  ((&((retval)  # "sllb" ->ₛ "head")) # Ptr  |-> retval_2)
   **  ((&((retval)  # "sllb" ->ₛ "ptail")) # Ptr  |-> &((retval)  # "sllb" ->ₛ "head"))
 |--
-  [| (0 = 0) |] 
+  [| (retval <> 0) |] 
+  &&  [| (0 = 0) |] 
   &&  [| (&((retval)  # "sllb" ->ₛ "head") = &((retval)  # "sllb" ->ₛ "head")) |] 
   &&  [| (retval_2 = 0) |] 
   &&  [| (retval <> 0) |]
@@ -289,7 +291,8 @@ Definition nil_list_box_partial_solve_wit_3 := nil_list_box_partial_solve_wit_3_
 
 Definition nil_list_box_which_implies_wit_1 := 
 forall (box: Z) (box_head: Z) (box_ptail: Z) ,
-  [| (box_head = 0) |] 
+  [| (box <> 0) |] 
+  &&  [| (box_head = 0) |] 
   &&  [| (box_ptail = &((box)  # "sllb" ->ₛ "head")) |]
   &&  ((&((box)  # "sllb" ->ₛ "head")) # Ptr  |-> box_head)
   **  ((&((box)  # "sllb" ->ₛ "ptail")) # Ptr  |-> box_ptail)
@@ -302,7 +305,8 @@ forall (box: Z) (box_head: Z) (box_ptail: Z) ,
 
 Definition cons_list_box_return_wit_1 := 
 forall (box_pre: Z) (data_pre: Z) (l: (@list Z)) (pt: Z) (retval: Z) ,
-  [| (pt = &((box_pre)  # "sllb" ->ₛ "head")) |]
+  [| (pt = &((box_pre)  # "sllb" ->ₛ "head")) |] 
+  &&  [| (box_pre <> 0) |]
   &&  (sll retval (cons (data_pre) (l)) )
   **  ((&((box_pre)  # "sllb" ->ₛ "head")) # Ptr  |-> retval)
   **  ((&((box_pre)  # "sllb" ->ₛ "ptail")) # Ptr  |-> &((retval)  # "sll" ->ₛ "next"))
@@ -312,7 +316,8 @@ forall (box_pre: Z) (data_pre: Z) (l: (@list Z)) (pt: Z) (retval: Z) ,
 
 Definition cons_list_box_return_wit_2 := 
 forall (box_pre: Z) (data_pre: Z) (l: (@list Z)) (pt: Z) (retval: Z) ,
-  [| (pt <> &((box_pre)  # "sllb" ->ₛ "head")) |]
+  [| (pt <> &((box_pre)  # "sllb" ->ₛ "head")) |] 
+  &&  [| (box_pre <> 0) |]
   &&  (sll retval (cons (data_pre) (l)) )
   **  ((&((box_pre)  # "sllb" ->ₛ "head")) # Ptr  |-> retval)
   **  ((&((box_pre)  # "sllb" ->ₛ "ptail")) # Ptr  |-> pt)
@@ -329,11 +334,13 @@ forall (box_pre: Z) (l: (@list Z)) ,
 
 Definition cons_list_box_partial_solve_wit_2 := 
 forall (box_pre: Z) (l: (@list Z)) (pt: Z) (h: Z) ,
-  ((&((box_pre)  # "sllb" ->ₛ "head")) # Ptr  |-> h)
+  [| (box_pre <> 0) |]
+  &&  ((&((box_pre)  # "sllb" ->ₛ "head")) # Ptr  |-> h)
   **  ((&((box_pre)  # "sllb" ->ₛ "ptail")) # Ptr  |-> pt)
   **  (sll h l )
 |--
-  (sll h l )
+  [| (box_pre <> 0) |]
+  &&  (sll h l )
   **  ((&((box_pre)  # "sllb" ->ₛ "head")) # Ptr  |-> h)
   **  ((&((box_pre)  # "sllb" ->ₛ "ptail")) # Ptr  |-> pt)
 .
@@ -343,7 +350,8 @@ forall (l: (@list Z)) (box: Z) ,
   (sllb box l )
 |--
   EX (pt: Z)  (h: Z) ,
-  ((&((box)  # "sllb" ->ₛ "head")) # Ptr  |-> h)
+  [| (box <> 0) |]
+  &&  ((&((box)  # "sllb" ->ₛ "head")) # Ptr  |-> h)
   **  ((&((box)  # "sllb" ->ₛ "ptail")) # Ptr  |-> pt)
   **  (sll h l )
 .
@@ -352,7 +360,8 @@ forall (l: (@list Z)) (box: Z) ,
 
 Definition map_list_box_return_wit_1 := 
 forall (x_pre: Z) (box_pre: Z) (l: (@list Z)) (pt: Z) (h: Z) ,
-  (sll h (map_mult (x_pre) (l)) )
+  [| (box_pre <> 0) |]
+  &&  (sll h (map_mult (x_pre) (l)) )
   **  ((&((box_pre)  # "sllb" ->ₛ "head")) # Ptr  |-> h)
   **  ((&((box_pre)  # "sllb" ->ₛ "ptail")) # Ptr  |-> pt)
 |--
@@ -368,11 +377,13 @@ forall (box_pre: Z) (l: (@list Z)) ,
 
 Definition map_list_box_partial_solve_wit_2 := 
 forall (box_pre: Z) (l: (@list Z)) (pt: Z) (h: Z) ,
-  ((&((box_pre)  # "sllb" ->ₛ "head")) # Ptr  |-> h)
+  [| (box_pre <> 0) |]
+  &&  ((&((box_pre)  # "sllb" ->ₛ "head")) # Ptr  |-> h)
   **  ((&((box_pre)  # "sllb" ->ₛ "ptail")) # Ptr  |-> pt)
   **  (sll h l )
 |--
-  (sll h l )
+  [| (box_pre <> 0) |]
+  &&  (sll h l )
   **  ((&((box_pre)  # "sllb" ->ₛ "head")) # Ptr  |-> h)
   **  ((&((box_pre)  # "sllb" ->ₛ "ptail")) # Ptr  |-> pt)
 .
@@ -382,7 +393,8 @@ forall (l: (@list Z)) (box: Z) ,
   (sllb box l )
 |--
   EX (pt: Z)  (h: Z) ,
-  ((&((box)  # "sllb" ->ₛ "head")) # Ptr  |-> h)
+  [| (box <> 0) |]
+  &&  ((&((box)  # "sllb" ->ₛ "head")) # Ptr  |-> h)
   **  ((&((box)  # "sllb" ->ₛ "ptail")) # Ptr  |-> pt)
   **  (sll h l )
 .
@@ -1035,8 +1047,8 @@ forall (l: (@list Z)) (box: Z) ,
 
 Module Type VC_Correct.
 
-Include common_Strategy_Correct.
 Include sll_project_Strategy_Correct.
+Include common_Strategy_Correct.
 
 Axiom proof_of_nil_list_safety_wit_1 : nil_list_safety_wit_1.
 Axiom proof_of_nil_list_return_wit_1 : nil_list_return_wit_1.
